finished a first draw of the encode proof

src/encode.v
@@ -11,53 +11,71 @@ Check n_bit_dont_fail.
 (* (* TODO :: Here this function can't be call for immediate *) *)
 Definition operand_to_bin (o : operande) : option (list bool) :=
   match o with
-    | imm_o (imm k) => n_bit 8 (k mod 256)
-    | reg_o (reg k) => n_bit 8 (k mod 256)
+    | imm_o (imm k) => n_bit 8 k
+    | reg_o (reg k) => n_bit 8 k
   end.
 
-Lemma operand_to_bin_never_fail : forall (o : operande), exists (l : list bool), operand_to_bin o = Some l.
+(* Lemma operand_to_bin_never_fail : forall (o : operande), exists (l : list bool), operand_to_bin o = Some l. *)
+(* Proof. *)
+(*   intros. *)
+(*   (* assert (forall (n : nat), n mod 256 <? 2 ^ 8 = true). *) *)
+(*   (* { *) *)
+(*     assert (forall (n : nat), n mod 256 < 2 ^ 8). *)
+(*     { *)
+(*       assert (2 ^ 8 = 256) by reflexivity. *)
+(*       rewrite H. *)
+(*       (* i need something of the form  "_ mod n < n" *) *)
+(*       Check Nat.mod_bound_pos. *)
+(*       intros n. *)
+(*       apply Nat.mod_bound_pos. *)
+(*       Search (0 <= _). *)
+(*       apply Peano.le_0_n. *)
+(*       Search (0 < S _). *)
+(*       apply Nat.lt_0_succ. *)
+(*     } *)
+(*     (* SearchAbout (_ < _). *) *)
+(*     (* intros. *) *)
+(*     (* specialize (Nat.ltb_spec0 (n mod 256) (2 ^ 8)). *) *)
+(*     (* intros. *) *)
+(*     (* apply reflect_iff in H0. *) *)
+(*     (* rewrite iff_to_and in H0. *) *)
+(*     (* destruct H0. *) *)
+(*     (* apply H0. *) *)
+(*     (* specialize (H n). *) *)
+(*     (* exact H. *) *)
+(*   (* }  *) *)
+(*   destruct o. *)
+(*   -unfold operand_to_bin. *)
+(*    destruct i. *)
+(*    apply n_bit_dont_fail. *)
+(*    specialize (H n). *)
+(*    exact H. *)
+(*   -unfold operand_to_bin. *)
+(*    destruct r. *)
+(*    apply n_bit_dont_fail. *)
+(*    specialize (H n). *)
+(*    exact H. *)
+(* Qed. *)
+(* SearchAbout bit_n. *)
+Lemma operand_to_bin_hypothesis1 : forall (l : list bool) (i : instruction_tern_n),
+    operand_to_bin (reg_o (instr_operande1_t_n i)) = Some l -> reg (bit_n l) = i.(instr_operande1_t_n).
 Proof.
   intros.
-  (* assert (forall (n : nat), n mod 256 <? 2 ^ 8 = true). *)
-  (* { *)
-    assert (forall (n : nat), n mod 256 < 2 ^ 8).
-    {
-      assert (2 ^ 8 = 256) by reflexivity.
-      rewrite H.
-      (* i need something of the form  "_ mod n < n" *)
-      Check Nat.mod_bound_pos.
-      intros n.
-      apply Nat.mod_bound_pos.
-      Search (0 <= _).
-      apply Peano.le_0_n.
-      Search (0 < S _).
-      apply Nat.lt_0_succ.
-    }
-    (* SearchAbout (_ < _). *)
-    (* intros. *)
-    (* specialize (Nat.ltb_spec0 (n mod 256) (2 ^ 8)). *)
-    (* intros. *)
-    (* apply reflect_iff in H0. *)
-    (* rewrite iff_to_and in H0. *)
-    (* destruct H0. *)
-    (* apply H0. *)
-    (* specialize (H n). *)
-    (* exact H. *)
-  (* }  *)
-  destruct o.
-  -unfold operand_to_bin.
-   destruct i.
-   apply n_bit_dont_fail.
-   specialize (H n).
-   exact H.
-  -unfold operand_to_bin.
-   destruct r.
-   apply n_bit_dont_fail.
-   specialize (H n).
-   exact H.
+  unfold operand_to_bin in H.
+  destruct (instr_operande1_t_n i).
+  Search n_bit.
+  apply n_bit_n in H.
+  rewrite H.
+  reflexivity.
 Qed.
 
+Lemma operand_to_bin_hypothesis2 : forall (l : list bool) (i : instruction_tern_n),
+    operand_to_bin (reg_o (instr_operande2_t_n i)) = Some l -> reg (bit_n l) = i.(instr_operande2_t_n).
+Admitted.
 
+Lemma operand_to_bin_hypothesis3 : forall (l : list bool) (i : instruction_tern_n),
+    operand_to_bin (reg_o (instr_operande3_t_n i)) = Some l -> reg (bit_n l) = i.(instr_operande3_t_n).
+Admitted.
 
 Lemma operand_to_bin_size : forall (o : operande) (l : list bool),
     operand_to_bin o = Some l -> length l = 8.
@@ -98,20 +116,50 @@ Compute get_first_n_bit testList' 3.
 Compute get_first_n_bit testList' 4.
 
 
-Lemma get_first_n_bit_size : forall (l : list bool) (n : nat), length l = n -> get_first_n_bit l n = (l,[]).
-Proof.
-  intros.
-  Admitted.
+  (* { *)
+  (*   assert (forall (l1 l2 l3 l4 l: list bool), l1 ++ l2 ++ l3 ++ l4 = l1 ++ l /\ l = l2 ++ l3 ++ l4) by admit. *)
+  (*   assert (forall (l1 l2 l3 l4 : list bool), length l1 = 8 -> get_first_n_bit (l1 ++ l2 ++ l3 ++ l4) 8 = (l1,l2 ++ l3 ++ l4)). *)
+  (*   { *)
+  (*     intros. *)
+  (*   } *)
 
-Lemma get_first_n_bit_size_tl : forall (l : list bool) (tl : list bool), length l = 8 -> get_first_n_bit (l ++ tl) 8 = (l,tl).
+
+Lemma get_first_n_bit_size_nil_n : forall (n : nat) (l : list bool), length l = n -> get_first_n_bit l n = (l,[]).
 Proof.
-  intros.
+  induction n.
+  -intros.
+   Search (length _ = 0).
+   apply length_zero_iff_nil in H.
+   rewrite H.
+   reflexivity.
+  -intros.
+   Search (length _ = S _).
+Admitted.
+   
+ 
+
+Lemma get_first_n_bit_size_tl : forall (tl : list bool) (l : list bool), length l = 8 -> get_first_n_bit (l ++ tl) 8 = (l,tl).
+Proof.
   induction tl.
-  -rewrite app_nil_r.
-   apply get_first_n_bit_size.
+  -intros.
+   rewrite app_nil_r.
+   apply get_first_n_bit_size_nil_n.
    exact H.
+  -
 Admitted.
 
+Lemma concat_3 : forall (l1 l2 l3: list bool), l1 ++ l2 ++ l3 = l1 ++ (l2 ++ l3).
+Proof.
+  intros.
+  
+Lemma concat_future : forall (l1 l2 l3 l4 : list bool), l1 ++ l2 ++ l3 ++ l4 
+
+Lemma get_first_n_bit_size_4 : forall (l1 l2 l3 l4 : list bool),
+    length l1 = 8 -> get_first_n_bit (l1 ++ l2 ++ l3 ++ l4) 8 = (l1,l2 ++ l3 ++ l4).
+Proof.
+  Search (_ ++ _ = _ ++ _).
+  
+  Admitted.
 
 (* Lemma get_first_n_bit_size : forall (bi : list bool) (size : nat), n < (length bi) -> get_first_n_bit bi n = ( *)
 
@@ -170,167 +218,6 @@ Definition encode_t_n (i : instruction_tern_n) : option binary_instruction :=
                                  fun o2 => let! o3 := operand_to_bin (reg_o i.(instr_operande3_t_n)) in
                                            fun o3 => ret (code ++ o1 ++ o2 ++ o3).
                                                          
-(* Definition encode (i : instruction) : option binary_instruction :=   *)
-(*   let! k := lookup i.(instr_opcode) encdec in *)
-(*   fun k => let! code := n_bit 8 k in *)
-(*            fun code => let! o1 := operand_to_bin i.(instr_operande1) in  *)
-(*                        fun o1 => let! o2 := operand_to_bin i.(instr_operande2) in *)
-(*                                  fun o2 =>                                             *)
-(*                                                let! o3 := compute_op3 i in                                               *)
-(*                                                fun o3 => ret (code ++ o1 ++ o2 ++ o3). *)
-
-
-(* Theorem encode_size : forall (i : instruction) (bi : binary_instruction), encode i = Some bi -> length bi = 32. *)
-(* Proof. *)
-(*   intros. *)
-(*   unfold encode in H. *)
-(*   intros. *)
-(*   unfold encode in H. *)
-(*   apply bind_rewrite in H. *)
-(*   destruct H. *)
-(*   destruct H. *)
-(*   apply bind_rewrite in H. *)
-(*   destruct H. *)
-(*   destruct H. *)
-(*   apply bind_rewrite in H. *)
-(*   destruct H. *)
-(*   destruct H. *)
-(*   apply bind_rewrite in H. *)
-(*   destruct H. *)
-(*   destruct H. *)
-(*   apply bind_rewrite in H. *)
-(*   destruct H. *)
-(*   destruct H. *)
-(*   Search operand_to_bin. *)
-(*   apply commut_equal in H4. *)
-(*   apply commut_equal in H3. *)
-(*   apply commut_equal in H2. *)
-(*   apply commut_equal in H1. *)
-(*   apply commut_equal in H0. *)
-(*   apply operand_to_bin_size in H3. *)
-(*   apply operand_to_bin_size in H2. *)
-(*   assert (keep : lookup (instr_opcode i) encdec = Some x) by auto. *)
-(*   assert (forall (t : tag) (n : nat), lookup t encdec = Some n -> n <= 3) by admit. *)
-(*   apply H5 in H0. *)
-(*   Search n_bit. *)
-(*   Check size_n_bit. *)
-(*   apply size_n_bit in H1. *)
-(*   apply compute_op3_size in H4. *)
-(*   assert (length x0 = 8 -> length x1 = 8 -> length x2 = 8 -> length x3 = 8 -> length (x0 ++ x1 ++ x2 ++ x3) = 32). *)
-(*   { *)
-(*     intros. *)
-(*     Search length. *)
-(*     Check app_length. *)
-(*     repeat (rewrite app_length). *)
-(*     rewrite H6. *)
-(*     rewrite H7. *)
-(*     rewrite H8. *)
-(*     rewrite H9. *)
-(*     reflexivity. *)
-(*   } *)
-(*   rewrite ret_rewrite in H. *)
-(*   inversion H. *)
-(*   auto. *)
-(* Admitted. *)
-
-(* Definition encode_mytho (i : instruction) : option (list bool) := *)
-(*   let! bo1 := lookup i.(instr_opcode) encdec in *)
-(*   fun bo1 => (n_bit 8 bo1). *)
-
-(* Definition decode_mytho (bi : list bool) : option tag := *)
-(*   match get_first_n_bit bi 8 with *)
-(*   | (h,tl) => lookdown (bit_n h) encdec *)
-(*   end. *)
-
-(* Definition my_instr_encoded_decoded := match encode_mytho my_instr with *)
-(*                                       | Some lol => decode_mytho lol *)
-(*                                       | None => None *)
-(*                                        end. *)
-
-(* Compute my_instr_encoded_decoded. *)
-
-(* Theorem test_theorem_mytho : forall (i : instruction) (bi : list bool), *)
-(*     encode_mytho i = Some bi -> decode_mytho bi = Some i.(instr_opcode). *)
-(* Proof. *)
-(*   intros i bi H. *)
-(*   unfold encode_mytho in H.   *)
-(*   apply bind_rewrite in H. *)
-(*   destruct H. *)
-(*   destruct H. *)
-(*   unfold decode_mytho. *)
-(*   assert (length bi = 8 -> get_first_n_bit bi 8 = (bi,[])). *)
-(*   { *)
-(*     intros. *)
-(*     admit. *)
-(*   } *)
-(*   assert (keep : n_bit 8 x = Some bi) by auto. *)
-(*   Check operand_to_bin_size. *)
-(*   specialize size_n_bit. *)
-(*   intros.   *)
-(*   apply H2 in H. *)
-(*   apply H1 in H. *)
-(*   rewrite H. *)
-(*   Search lookdown. *)
-(*   apply lookdup_encdec. *)
-(*   unfold lookdown. *)
-(*   assert (n_bit 8 x = Some bi -> bit_n bi = x). *)
-(*   { *)
-(*     intros. *)
-(*     Search n_bit. *)
-(*     specialize (n_bit_n bi 8 x). *)
-(*     intros. *)
-(*     apply H4 in H3. *)
-(*     exact H3. *)
-(*   } *)
-(*   rewrite H3. *)
-(*   -apply commut_equal. *)
-(*    exact H0. *)
-(*   -exact keep. *)
-(* Admitted. *)
-  
-  
-  
-
-
-
-
-
-(* this is test purpose *)
-(* Definition encode_mytho (i : instruction) : option binary_instruction := *)
-(*   let! bo1 := operand_to_bin i.(instr_operande1) in *)
-(*   fun bo1 => ret bo1. *)
-
-(* Definition decode_mytho (bi : binary_instruction) : option instruction := *)
-(*   match get_first_n_bit with *)
-(*   | (h,tl) => bit_n h  *)
-
-(* Print operand_to_bin. *)
-
-(* Lemma test_proof : forall (i : instruction) (l : list bool) (bi : binary_instruction), encode_mytho i = Some bi -> length bi = 8. *)
-(* Proof. *)
-(*   intros. *)
-(*   unfold encode_mytho in H. *)
-(*   Check bind_rewrite. *)
-(*   specialize bind_rewrite. *)
-(*   intros. *)
-(*   apply H0 in H. *)
-(*   destruct H. *)
-(*   destruct H. *)
-(*   specialize (ret_rewrite (list bool)). *)
-(*   intros. *)
-(*   rewrite H2 in H. *)
-(*   inversion H. *)
-(*   specialize (commut_equal (option (list bool))). *)
-(*   intros. *)
-(*   apply H3 in H1. *)
-(*   Check operand_to_bin_size. *)
-(*   apply operand_to_bin_size in H1.   *)
-(*   rewrite <- H4. *)
-(*   exact H1. *)
-(* Qed. *)
-
-
-
 
 
   (* flux d'instruction il faut faire une fonction qui decode le debut de la liste et retourne la suite de la liste *)
@@ -367,125 +254,184 @@ Definition decode (bi : binary_instruction) : option instruction :=
   end.
 
 
-                                                                            
 
-Definition decode (bi : binary_instruction) : option instruction :=
-  match get_first_n_bit bi 8 with
-  | (li,next) => let! t := lookdown (bit_n li) encdec in
-                 fun t => match get_first_n_bit next 8 with
-                          | (op1,next) => match get_first_n_bit next 8 with
-                                          | (op2,next) => match get_first_n_bit next 8 with
-                                                          | (op3,next) => match t with
-                                                                          | tag_n tn => Some (mk_instr t
-                                                                                                       (reg (bit_n op1))
-                                                                                                       (reg (bit_n  op2))
-                                                                                                       (reg (bit_n  op3)))
-                                                                          | tag_i ti => Some (mk_instr t
-                                                                                                       (reg (bit_n op1))
-                                                                                                       (reg (bit_n op2))
-                                                                                                       (immediate (bit_n op3)))
-                                                                          end
-                                                          end
-                                          end
-                          end
-  end.
+Definition my_instr := (mk_instr_t_n AND (reg 10) (reg 11) (reg 12)).
 
 
-Print my_instr.
-Definition my_instr_encoded_decoded' := match encode my_instr with
+Definition my_instr_encoded_decoded' := match encode_t_n my_instr with
                                       | Some lol => decode lol
                                       | None => None
-                                       end.
+                                       end. 
 Print my_instr.
-Compute my_instr_encoded_decoded.
+Compute my_instr_encoded_decoded'.
+
+(* this is an important thinking i have to try to find this relation into my proof *)
+(* Lemma decode_rewrite_inst_t_n : forall (i : instruction_tern_n) (bi : binary_instruction), *)
+(*     decode bi = Some (instr_t_n i) -> i.(instr_opcode_t_n) = (lookdown (bit_n (get_first_n_bit bi 8)) encdec). *)
+
+
+Lemma encode_decode_t_n : forall (i : instruction_tern_n) (bi : binary_instruction),
+    encode_t_n i = Some bi -> decode bi = Some (instr_t_n i).
+Proof.
+  intros.
+  unfold encode_t_n in H.
+  apply bind_rewrite in H.
+  destruct H.
+  destruct H.
+  apply bind_rewrite in H.
+  destruct H.
+  destruct H.
+  apply bind_rewrite in H.
+  destruct H.
+  destruct H.
+  apply bind_rewrite in H.
+  destruct H.
+  destruct H.
+  apply bind_rewrite in H.
+  destruct H.
+  destruct H.
+  unfold decode.
+  rewrite ret_rewrite in H.
+  inversion H.  
+  assert (length x0 = 8) by (apply commut_equal in H1; apply size_n_bit in H1; auto).
+  assert (get_first_n_bit (x0 ++ x1 ++ x2 ++ x3) 8 = (x0,x1 ++ x2 ++ x3)).
+  {
+    
+    admit.
+  }
+  rewrite H7.
+  apply commut_equal in H0.
+  Search lookup.
+  apply lookup_encdecP in H0.
+  apply commut_equal in H1.
+  assert (bit_n x0 = x).
+  {
+    apply n_bit_n in H1.
+    exact H1.
+  }
+  rewrite H8.
+  rewrite H0.
+  assert (forall (f : tag -> (option instruction)), bind (Some (tag_t_n (instr_opcode_t_n i))) f = f (tag_t_n (instr_opcode_t_n i))) by reflexivity.
+  rewrite H9.
+  assert (get_first_n_bit  (x1 ++ x2 ++ x3) 8 = (x1,x2 ++ x3)) by admit.
+  rewrite H10.
+  assert (get_first_n_bit  (x2 ++ x3) 8 = (x2,x3)) by admit.
+  rewrite H11.
+  assert (get_first_n_bit  (x3) 8 = (x3,[])) by admit.
+  rewrite H12.
+  rewrite ret_rewrite. 
+  Check operand_to_bin_hypothesis1.
+  apply commut_equal in H2.
+  apply operand_to_bin_hypothesis1 in H2.
+  rewrite H2.
+  apply commut_equal in H3.
+  apply operand_to_bin_hypothesis2 in H3.
+  rewrite H3.
+  apply commut_equal in H4.
+  apply operand_to_bin_hypothesis3 in H4.
+  rewrite H4.
+
+  
+  assert ({|
+       instr_opcode_t_n := instr_opcode_t_n i;
+       instr_operande1_t_n := instr_operande1_t_n i;
+       instr_operande2_t_n := instr_operande2_t_n i;
+       instr_operande3_t_n := instr_operande3_t_n i |} = i).
+  {
+    simpl. destruct i.
+    compute. reflexivity.
+  }
+  rewrite H13.
+  reflexivity.
+  
 
 Check instruction.
 
 
 
 
-Theorem encode_decode : forall (i : instruction) (bi : binary_instruction), encode i = Some bi -> decode bi = Some i.
-Proof.
-  assert (I: forall (i : instruction) (bi : binary_instruction), encode i = Some bi -> decode bi = Some i).
-  {
-    intros.
-    unfold encode in H.
-    apply bind_rewrite in H.
-    destruct H.
-    destruct H.
-    apply bind_rewrite in H.
-    destruct H.
-    destruct H.
-    apply bind_rewrite in H.
-    destruct H.
-    destruct H.
-    apply bind_rewrite in H.
-    destruct H.
-    destruct H.
-    apply bind_rewrite in H.
-    destruct H.
-    destruct H.
-    Check get_first_n_bit_size_tl.
-    Search ret.
-    rewrite ret_rewrite in H.
-    inversion H.
-    Check get_first_n_bit_size_tl.
-    assert (length x0 = 8 -> get_first_n_bit (x0 ++ x1 ++ x2 ++ x3) 8 = (x0, x1 ++ x2 ++ x3)) by admit.    
-    unfold decode.
-    rewrite H5.
-    -{
-        apply commut_equal in H0.
-        apply lookdup_encdec in H0.
-        Search n_bit.
-        Check bit_n_bit.
-        apply commut_equal in H1.
-        apply n_bit_n in H1.
-        rewrite H1.
-        rewrite H0.
-        assert (forall (f : tag -> option instruction), bind (Some (instr_opcode i)) f = f (instr_opcode i)) by reflexivity.
-        rewrite H7.
-        assert(get_first_n_bit (x1 ++ x2 ++ x3) 8 = (x1,x2 ++ x3)) by admit.
-        rewrite H8.
-        assert(get_first_n_bit (x2 ++ x3) 8 = (x2,x3)) by admit.
-        rewrite H9.
-        assert(get_first_n_bit x3 8 = (x3,[])) by admit.
-        rewrite H10.
-        destruct (instr_opcode i).        
-        -{
-            admit.
-          }
-        -
-  }
-Admitted.
+(* Theorem encode_decode : forall (i : instruction) (bi : binary_instruction), encode i = Some bi -> decode bi = Some i. *)
+(* Proof. *)
+(*   assert (I: forall (i : instruction) (bi : binary_instruction), encode i = Some bi -> decode bi = Some i). *)
+(*   { *)
+(*     intros. *)
+(*     unfold encode in H. *)
+(*     apply bind_rewrite in H. *)
+(*     destruct H. *)
+(*     destruct H. *)
+(*     apply bind_rewrite in H. *)
+(*     destruct H. *)
+(*     destruct H. *)
+(*     apply bind_rewrite in H. *)
+(*     destruct H. *)
+(*     destruct H. *)
+(*     apply bind_rewrite in H. *)
+(*     destruct H. *)
+(*     destruct H. *)
+(*     apply bind_rewrite in H. *)
+(*     destruct H. *)
+(*     destruct H. *)
+(*     Check get_first_n_bit_size_tl. *)
+(*     Search ret. *)
+(*     rewrite ret_rewrite in H. *)
+(*     inversion H. *)
+(*     Check get_first_n_bit_size_tl. *)
+(*     assert (length x0 = 8 -> get_first_n_bit (x0 ++ x1 ++ x2 ++ x3) 8 = (x0, x1 ++ x2 ++ x3)) by admit.     *)
+(*     unfold decode. *)
+(*     rewrite H5. *)
+(*     -{ *)
+(*         apply commut_equal in H0. *)
+(*         apply lookdup_encdec in H0. *)
+(*         Search n_bit. *)
+(*         Check bit_n_bit. *)
+(*         apply commut_equal in H1. *)
+(*         apply n_bit_n in H1. *)
+(*         rewrite H1. *)
+(*         rewrite H0. *)
+(*         assert (forall (f : tag -> option instruction), bind (Some (instr_opcode i)) f = f (instr_opcode i)) by reflexivity. *)
+(*         rewrite H7. *)
+(*         assert(get_first_n_bit (x1 ++ x2 ++ x3) 8 = (x1,x2 ++ x3)) by admit. *)
+(*         rewrite H8. *)
+(*         assert(get_first_n_bit (x2 ++ x3) 8 = (x2,x3)) by admit. *)
+(*         rewrite H9. *)
+(*         assert(get_first_n_bit x3 8 = (x3,[])) by admit. *)
+(*         rewrite H10. *)
+(*         destruct (instr_opcode i).         *)
+(*         -{ *)
+(*             admit. *)
+(*           } *)
+(*         - *)
+(*   } *)
+(* Admitted. *)
 
 
 
 
 
-Lemma encode_decode : forall (i : instruction) (bi : binary_instruction), encode i = Some bi -> decode bi = Some i.
-Proof.
-  (* why can't i write this ? *)
-(*   assert (I : forall (i : instruction) (bi : binary_instruction), encode i = Some bi ->
-                                                                  lookdown (bit_n (cut_binary_instruction bi 0 8)) = (i.instr_opcode)). *)
-  induction i.
-  unfold encode.
+(* Lemma encode_decode : forall (i : instruction) (bi : binary_instruction), encode i = Some bi -> decode bi = Some i. *)
+(* Proof. *)
+(*   (* why can't i write this ? *) *)
+(* (*   assert (I : forall (i : instruction) (bi : binary_instruction), encode i = Some bi -> *)
+(*                                                                   lookdown (bit_n (cut_binary_instruction bi 0 8)) = (i.instr_opcode)). *) *)
+(*   induction i. *)
+(*   unfold encode. *)
 
   
   
-Admitted.
+(* Admitted. *)
 
 
 
 
 
-Example test_instr := mk_instr (tag_i ADD_I) (reg 10) (reg 11) (immediate 12).
-Compute encode test_instr.
-Definition testBoolList := [false; true; false; false; false; false; false; false; false; true; false; true; false; false; false; false; true; true; false; true; false; false; false; false; false; false; true; true; false; false; false; false].
-Compute length testBoolList.
+(* Example test_instr := mk_instr (tag_i ADD_I) (reg 10) (reg 11) (immediate 12). *)
+(* Compute encode test_instr. *)
+(* Definition testBoolList := [false; true; false; false; false; false; false; false; false; true; false; true; false; false; false; false; true; true; false; true; false; false; false; false; false; false; true; true; false; false; false; false]. *)
+(* Compute length testBoolList. *)
 
-encode test_instr
+(* encode test_instr *)
 
-Compute (match encode test_instr with | Some i => decode i | None => None end).
+(* Compute (match encode test_instr with | Some i => decode i | None => None end). *)
   
 
 
